Using Functional Arrays as definitions of Slices

proof-libs/fstar/core/Alloc.Vec.fst
@@ -3,10 +3,10 @@ open Rust_primitives
 
 unfold type t_Vec t (_: unit) = t_Slice t
 
-let impl__new #t (): t_Vec t () = FStar.Seq.empty
+let impl__new #t (): t_Vec t () = empty
 
-let impl_2__extend_from_slice #t (#[(Tactics.exact (`()))]alloc:unit) (self: t_Vec t alloc) (other: t_Slice t{Seq.length self + Seq.length other <= max_usize}): t_Vec t alloc
-  = FStar.Seq.append self other
+let impl_2__extend_from_slice #t (#[(Tactics.exact (`()))]alloc:unit) (self: t_Vec t alloc) (other: t_Slice t{v (length self) + v (length other) <= max_usize}): t_Vec t alloc
+  = concat self other
 
 let impl__with_capacity (_capacity: usize) = impl__new ()
 
@@ -15,16 +15,14 @@ let impl__with_capacity (_capacity: usize) = impl__new ()
 // instead.
 let impl_1__push #t
   (#[(Tactics.exact (`()))]alloc:unit)
-  (v: t_Vec t alloc)// Removed: {Seq.length v + 1 <= max_usize})
+  (v: t_Vec t alloc)
   (x: t)
    : t_Vec t alloc = 
-     if Seq.length v >= max_usize then v else
-     FStar.Seq.append v (FStar.Seq.create 1 x)
+     if length v = sz (max_usize) then v else
+     concat v (create (sz 1) x)
 
 let impl_1__len #t (#[(Tactics.exact (`()))]alloc:unit) (v: t_Vec t alloc) =
-  let n = Seq.length v in
-  assert (n <= maxint usize_inttype);
-  mk_int #usize_inttype (Seq.length v)
+  length v
 
 let impl_1__as_slice #t (#[(Tactics.exact (`()))]alloc:unit) (v: t_Vec t alloc) : t_Slice t = v
 
@@ -34,19 +32,19 @@ open Rust_primitives.Hax
 open Core.Ops.Index
 instance update_at_tc_array t n: update_at_tc (t_Vec t ()) (int_t n) = {
   super_index = FStar.Tactics.Typeclasses.solve <: t_Index (t_Vec t ()) (int_t n);
-  update_at = (fun arr i x -> FStar.Seq.upd arr (v i) x);
+  update_at = (fun arr i x -> upd arr (sz (v i)) x);
 }
 
 
 let impl_1__is_empty #t (#[(Tactics.exact (`()))]alloc:unit) (v: t_Vec t alloc): bool =
-  Seq.length v = 0
+  length v = sz 0
 
 let impl_1__insert #t (#[(Tactics.exact (`()))]alloc:unit) (v: t_Vec t alloc) 
-  (index: usize {Rust_primitives.Integers.v index <= Seq.length v}) (element: t) =
-  let index = Rust_primitives.Integers.v #USIZE index in
-  let left = Seq.slice #t v 0 index in 
-  let right = Seq.slice #t v index (Seq.length v) in 
-  Seq.append left (Seq.cons element right)
+  (index: usize {index <=. length v /\ length v <. sz max_usize}) (element: t) 
+  : t_Vec t alloc =
+  let left = slice #t v (sz 0) index in 
+  let right = slice #t v index (length v) in 
+  concat left (cons element right)
 
 assume val impl_1__drain #t (#[(Tactics.exact (`()))]alloc:unit) #range_t  (v: t_Vec t alloc) (r: range_t): 
   t_Vec t alloc & Alloc.Vec.Drain.t_Drain t alloc
@@ -61,8 +59,8 @@ assume val impl_2__resize #t (#[(Tactics.exact (`()))]alloc:unit)  (v: t_Vec t a
       Prims.l_True
       (ensures
         fun new_v ->
-          Rust_primitives.v new_size ==
-          Seq.length new_v)
+          new_size ==
+          length new_v)
 
 assume val impl_1__remove #t (#[(Tactics.exact (`()))]alloc:unit)  (v: t_Vec t alloc) (index: usize): t_Vec t alloc & t
 
