proof-libs/fstar/core/Core.Slice.fsti
@@ -3,8 +3,8 @@ open Rust_primitives.Arrays
 open Rust_primitives.Integers
 
 let impl__len (#t: Type) (s: t_Slice t)
-  : len: usize {len == sz (Seq.length s)} = 
-  sz (Seq.length s)
+  : len: usize {len == length s} = 
+  length s
 
 open Core.Slice.Iter
 
@@ -23,22 +23,22 @@ instance impl__index t n: t_Index (t_Slice t) (int_t n)
   = { f_Output = t;
       f_index_pre = (fun (s: t_Slice t) (i: int_t n) -> v i >= 0 && v i < v (length s));
       f_index_post = (fun _ _ _ -> true);
-      f_index = (fun s i -> Seq.index s (v i));
+      f_index = (fun s i -> index s (sz (v i)));
     }
 
 let impl__copy_from_slice #t (x: t_Slice t) (y:t_Slice t) : t_Slice t = y
 let impl__clone_from_slice #t (x: t_Slice t) (y:t_Slice t) : t_Slice t = y
 
 val impl__split_at #t (s: t_Slice t) (mid: usize): Pure (t_Slice t * t_Slice t)
-    (requires (v mid <= Seq.length s))
-    (ensures (fun (x,y) -> Seq.length x == v mid /\ Seq.length y == Seq.length s - v mid /\
-                        x == Seq.slice s 0 (v mid) /\ y == Seq.slice s (v mid) (Seq.length s) /\
-                        s == Seq.append x y))
+    (requires (mid <=. length s))
+    (ensures (fun (x,y) -> length x == mid /\ length y == length s -. mid /\
+                        x == slice s (sz 0) mid /\ y == slice s mid (length s) /\
+                        s == concat x y))
 
-let impl__is_empty (s: t_Slice 'a): bool = Seq.length s = 0
+let impl__is_empty (s: t_Slice 'a): bool = length s = sz 0
 
 let impl__contains (#t: eqtype) (s: t_Slice t) (v: t) =
-  Seq.mem v s 
+  mem v s 
 
 val impl__copy_within
       (#v_T #v_R: Type0)
